src/Examples/HACMSDemo/WheelSensorEncoder.v
@@ -1,0 +1,107 @@
+Require Import Coq.Strings.Ascii
+        Coq.Bool.Bool
+        Coq.Lists.List
+        Coq.Structures.OrderedType.
+
+Require Import
+        Fiat.BinEncoders.Env.BinLib.Core
+        Fiat.BinEncoders.Env.Common.Specs
+        Fiat.BinEncoders.Env.Common.Compose
+        Fiat.BinEncoders.Env.Common.ComposeOpt
+        Fiat.BinEncoders.Env.Automation.Solver
+        Fiat.BinEncoders.Env.Lib2.WordOpt
+        Fiat.BinEncoders.Env.Lib2.NatOpt
+        Fiat.BinEncoders.Env.Lib2.StringOpt
+        Fiat.BinEncoders.Env.Lib2.EnumOpt
+        Fiat.BinEncoders.Env.Lib2.FixListOpt
+        Fiat.BinEncoders.Env.Lib2.SumTypeOpt.
+
+Require Import
+        Fiat.Common.SumType
+        Fiat.Examples.Tutorial.Tutorial
+        Fiat.Examples.DnsServer.DecomposeEnumField
+        Fiat.QueryStructure.Automation.AutoDB
+        Fiat.QueryStructure.Implementation.DataStructures.BagADT.BagADT
+        Fiat.QueryStructure.Automation.IndexSelection
+        Fiat.QueryStructure.Specification.SearchTerms.ListPrefix
+        Fiat.QueryStructure.Automation.SearchTerms.FindPrefixSearchTerms
+        Fiat.QueryStructure.Automation.MasterPlan
+        Fiat.Examples.HACMSDemo.DuplicateFree
+        Fiat.Examples.HACMSDemo.HACMSDemo
+        Fiat.Examples.HACMSDemo.WheelSensor.
+
+(* We first synthesize an implementation of our encoder. *)
+Lemma Sharpened_encode_SensorData_Impl
+  : { encode_SensorData_Impl : _ &
+      forall ce (val : SensorType),
+        refine (encode_SensorData_Spec val ce)
+               (ret (encode_SensorData_Impl val ce))}.
+Proof.
+  eexists; intros; set_evars.
+  unfold encode_SensorData_Spec.
+  unfold compose, Bind2.
+  setoid_rewrite refine_encode_enum; simplify with monad laws.
+  setoid_rewrite (@refine_encode_SumType
+          bin
+          _
+          2
+          ([nat : Type; nat : Type])
+          _
+          (icons _
+                 (icons _ (inil (A := Type))))).
+  simplify with monad laws.
+  simpl; rewrite app_nil_r.
+  finish honing.
+  simpl; f_equiv.
+  simpl; repeat apply Build_prim_and; eauto;
+    intros; rewrite refine_encode_nat; finish honing.
+Defined.
+
+(* Extract the synthesized encoder. *)
+Definition encode_SensorData_Impl :=
+  Eval simpl in projT1 Sharpened_encode_SensorData_Impl.
+
+(* Extract its proof of correctness for good measure. *)
+Lemma refine_encode_SensorData_Impl
+  : forall ce (val : SensorType),
+        refine (encode_SensorData_Spec val ce)
+               (ret (encode_SensorData_Impl val ce)).
+Proof.
+  exact (projT2 Sharpened_encode_SensorData_Impl).
+Qed.
+
+Opaque encode_SensorData_Spec.
+
+Theorem SharpenedWheelSensor :
+    FullySharpened WheelSensorSpec.
+Proof.
+  start sharpening ADT.
+  start_honing_QueryStructure'.
+  (* We first insert checks for the DuplicateFree constraints.  *)
+  hone method "AddSpeedSubscriber". { dropDuplicateFree. }
+  hone method "AddTirePressureSubscriber". { dropDuplicateFree. }
+  (* Break down the suscribers 'table' into one for each topic.  *)
+  decompose_EnumField "subscribers" "topic".
+  (* Select the kinds of searches each 'table' should support. *)
+  chooseIndexes.
+  (* Implement each method using the chosen search operations. *)
+  initializer.
+  insertOne.
+  insertOne.
+  rewrite refine_encode_SensorData_Impl; planOne.
+  rewrite refine_encode_SensorData_Impl; planOne.
+  (* Cleanup the synthesized methods. *)
+  final_optimizations.
+  (* Ensure the implementation is executable. *)
+  determinize.
+  (* Select concrete data structures for each table.  *)
+  choose_data_structures.
+  (* Some final cleanup. *)
+  final_simplification.
+  (* And we're done! *)
+  use_this_one.
+Defined.
+
+(* We can now extract the implementation derived above. *)
+Definition WheelSensorImpl := Eval simpl in projT1 SharpenedWheelSensor.
+Print WheelSensorImpl.
